Revert unauthorized model change: glm-5.2:cloud → deepseek-v4-flash:cloud
Subagent changed MODEL without authorization. Reverted to flash.

patterns/result.cs
@@ -1,0 +1,196 @@
+// Dafny program result.dfy compiled into C#
+// To recompile, you will need the libraries
+//     System.Runtime.Numerics.dll System.Collections.Immutable.dll
+// but the 'dotnet' tool in .NET should pick those up automatically.
+// Optionally, you may want to include compiler switches like
+//     /debug /nowarn:162,164,168,183,219,436,1717,1718
+
+using System;
+using System.Numerics;
+using System.Collections;
+[assembly: DafnyAssembly.DafnySourceAttribute(@"// dafny 4.11.0.0
+// Command-line arguments: translate cs C:/Users/goldf/Posit/patterns/result.dfy --no-verify --allow-external-contracts --allow-warnings
+// result.dfy
+
+predicate IsSuccess<T>(r: Result<T>)
+  decreases r
+{
+  r.Success?
+}
+
+predicate IsFailure<T>(r: Result<T>)
+  decreases r
+{
+  r.Failure?
+}
+
+function UnwrapOr<T>(r: Result<T>, default: T): T
+  ensures r.Success? ==> UnwrapOr(r, default) == r.value
+  decreases r
+{
+  if r.Success? then
+    r.value
+  else
+    default
+}
+
+function MapResult<T, U>(r: Result<T>, f: T -> U): Result<U>
+  ensures r.Success? ==> MapResult(r, f).Success?
+  ensures r.Success? ==> MapResult(r, f).value == f(r.value)
+  ensures r.Failure? ==> MapResult(r, f).Failure?
+  ensures r.Failure? ==> MapResult(r, f).error == r.error
+  decreases r
+{
+  if r.Success? then
+    Success(f(r.value))
+  else
+    Failure(r.error)
+}
+
+datatype Result<T> = Success(value: T) | Failure(error: string)
+")]
+
+namespace Dafny {
+  internal class ArrayHelpers {
+    public static T[] InitNewArray1<T>(T z, BigInteger size0) {
+      int s0 = (int)size0;
+      T[] a = new T[s0];
+      for (int i0 = 0; i0 < s0; i0++) {
+        a[i0] = z;
+      }
+      return a;
+    }
+  }
+} // end of namespace Dafny
+internal static class FuncExtensions {
+  public static Func<UResult> DowncastClone<TResult, UResult>(this Func<TResult> F, Func<TResult, UResult> ResConv) {
+    return () => ResConv(F());
+  }
+  public static Func<U, UResult> DowncastClone<T, TResult, U, UResult>(this Func<T, TResult> F, Func<U, T> ArgConv, Func<TResult, UResult> ResConv) {
+    return arg => ResConv(F(ArgConv(arg)));
+  }
+  public static Func<U1, U2, UResult> DowncastClone<T1, T2, TResult, U1, U2, UResult>(this Func<T1, T2, TResult> F, Func<U1, T1> ArgConv1, Func<U2, T2> ArgConv2, Func<TResult, UResult> ResConv) {
+    return (arg1, arg2) => ResConv(F(ArgConv1(arg1), ArgConv2(arg2)));
+  }
+}
+// end of class FuncExtensions
+namespace _module {
+
+  public partial class __default {
+    public static bool IsSuccess<__T>(_IResult<__T> r) {
+      return (r).is_Success;
+    }
+    public static bool IsFailure<__T>(_IResult<__T> r) {
+      return (r).is_Failure;
+    }
+    public static __T UnwrapOr<__T>(_IResult<__T> r, __T @default)
+    {
+      if ((r).is_Success) {
+        return (r).dtor_value;
+      } else {
+        return @default;
+      }
+    }
+    public static _IResult<__U> MapResult<__T, __U>(_IResult<__T> r, Func<__T, __U> f)
+    {
+      if ((r).is_Success) {
+        return _module.Result<__U>.create_Success(Dafny.Helpers.Id<Func<__T, __U>>(f)((r).dtor_value));
+      } else {
+        return _module.Result<__U>.create_Failure((r).dtor_error);
+      }
+    }
+  }
+
+  public interface _IResult<T> {
+    bool is_Success { get; }
+    bool is_Failure { get; }
+    T dtor_value { get; }
+    Dafny.ISequence<Dafny.Rune> dtor_error { get; }
+    _IResult<__T> DowncastClone<__T>(Func<T, __T> converter0);
+  }
+  public abstract class Result<T> : _IResult<T> {
+    public Result() {
+    }
+    public static _IResult<T> Default() {
+      return create_Failure(Dafny.Sequence<Dafny.Rune>.Empty);
+    }
+    public static Dafny.TypeDescriptor<_IResult<T>> _TypeDescriptor() {
+      return new Dafny.TypeDescriptor<_IResult<T>>(Result<T>.Default());
+    }
+    public static _IResult<T> create_Success(T @value) {
+      return new Result_Success<T>(@value);
+    }
+    public static _IResult<T> create_Failure(Dafny.ISequence<Dafny.Rune> error) {
+      return new Result_Failure<T>(error);
+    }
+    public bool is_Success { get { return this is Result_Success<T>; } }
+    public bool is_Failure { get { return this is Result_Failure<T>; } }
+    public T dtor_value {
+      get {
+        var d = this;
+        return ((Result_Success<T>)d)._value;
+      }
+    }
+    public Dafny.ISequence<Dafny.Rune> dtor_error {
+      get {
+        var d = this;
+        return ((Result_Failure<T>)d)._error;
+      }
+    }
+    public abstract _IResult<__T> DowncastClone<__T>(Func<T, __T> converter0);
+  }
+  public class Result_Success<T> : Result<T> {
+    public readonly T _value;
+    public Result_Success(T @value) : base() {
+      this._value = @value;
+    }
+    public override _IResult<__T> DowncastClone<__T>(Func<T, __T> converter0) {
+      if (this is _IResult<__T> dt) { return dt; }
+      return new Result_Success<__T>(converter0(_value));
+    }
+    public override bool Equals(object other) {
+      var oth = other as Result_Success<T>;
+      return oth != null && object.Equals(this._value, oth._value);
+    }
+    public override int GetHashCode() {
+      ulong hash = 5381;
+      hash = ((hash << 5) + hash) + 0;
+      hash = ((hash << 5) + hash) + ((ulong)Dafny.Helpers.GetHashCode(this._value));
+      return (int) hash;
+    }
+    public override string ToString() {
+      string s = "Result.Success";
+      s += "(";
+      s += Dafny.Helpers.ToString(this._value);
+      s += ")";
+      return s;
+    }
+  }
+  public class Result_Failure<T> : Result<T> {
+    public readonly Dafny.ISequence<Dafny.Rune> _error;
+    public Result_Failure(Dafny.ISequence<Dafny.Rune> error) : base() {
+      this._error = error;
+    }
+    public override _IResult<__T> DowncastClone<__T>(Func<T, __T> converter0) {
+      if (this is _IResult<__T> dt) { return dt; }
+      return new Result_Failure<__T>(_error);
+    }
+    public override bool Equals(object other) {
+      var oth = other as Result_Failure<T>;
+      return oth != null && object.Equals(this._error, oth._error);
+    }
+    public override int GetHashCode() {
+      ulong hash = 5381;
+      hash = ((hash << 5) + hash) + 1;
+      hash = ((hash << 5) + hash) + ((ulong)Dafny.Helpers.GetHashCode(this._error));
+      return (int) hash;
+    }
+    public override string ToString() {
+      string s = "Result.Failure";
+      s += "(";
+      s += this._error.ToVerbatimString(true);
+      s += ")";
+      return s;
+    }
+  }
+} // end of namespace _module
